$$
{\sum_{x\in A}}'f(x) {{\rm def}\atop =} \sum_{x\in A \atop x\ne 0}f(x)
$$

$$
{\sum_{x\in A}}'f(x) \vbox{\hbox{\rm def}\hbox{=}} \sum_{x\in A \atop x\ne 0}f(x)
$$


$$
{\sum_{x\in A}}'f(x) \vbox{\hbox{\rm def}\hbox{\hfil=\hfil}} \sum_{x\in A \atop x\ne 0}f(x)
$$


$$
{\sum_{x\in A}}'f(x) \vbox{\hbox{\rm def}\hbox{\rlap{\hphantom{\rm def}}\hfill=\hfill}} \sum_{x\in A \atop x\ne 0}f(x)
$$

$$
{\sum_{x\in A}}'f(x) {{{\scriptstyle \rm def}}\atop =} \sum_{{\scriptstyle x\in A} \atop {\scriptstyle x\ne 0}}f(x)
$$

$$
{\sum_{x\in A}}'f(x) =^{\rm def} \sum_{{\scriptstyle x\in A} \atop {\scriptstyle x\ne 0}}f(x)
$$

$$
{\sum_{x\in A}}'f(x) \mathop{=}\limits^{\rm def} \sum_{{\scriptstyle x\in A} \atop {\scriptstyle x\ne 0}}f(x)
$$

Answer

$$\mathop{{\sum}'}_{x\in A}f(x)\mathrel{\mathop=^{\rm def}}
\sum_{\scriptstyle x\in A\atop\scriptstyle x\ne0}f(x).$$


\end

